\section{Aufgabe 2}

Berechnen Sie den Wert der Reihe:
\begin{align*}
	\begin{array}{ l c }
		\text{a)} & \sum\limits _{k=0}^{\infty }\frac{2k+3}{k!}
	\end{array} & & \begin{array}{ l c }
		\text{b)} & \sum\limits _{k=0}^{\infty }\frac{k^{2} +4k-1}{k!}
	\end{array}
\end{align*}


\subsection{Lösung 2a}
\begin{equation*}
	\begin{array}{ c l }
		\sum\limits _{k=0}^{\infty }\frac{2k+3}{k!} & =\sum\limits _{k=0}^{\infty }\left(\frac{2}{( k-1) !} +\frac{3}{k!}\right)\\
		& =2\cdotp \sum\limits _{k=-1}^{\infty }\frac{1}{k!} +3\cdotp \sum\limits _{k=0}^{\infty }\frac{1}{k!}\\
		& =2\cdotp \sum\limits _{k=0}^{\infty }\frac{1}{k!} +\frac{2}{( -1) !} +3\cdotp \sum\limits _{k=0}^{\infty }\frac{1}{k!}\\
		& =2\cdotp e+0+3\cdotp e\\
		& =5e
	\end{array}
\end{equation*}

\subsection{Lösung 2b}
\begin{equation*}
	\begin{array}{ c l }
		\sum\limits _{k=0}^{\infty }\frac{k^{2} +4k-1}{k!} & =\\
		& 
	\end{array}
\end{equation*}
