\section*{Aufgabe 5}

Berechnen Sie die Grenzwerte:
\begin{align*}
  \begin{array}{ c c }
    \text{a)} & \lim\limits _{n\rightarrow \infty }\left(\left( 1-\frac{2}{n}\right)^{3n}\right)
  \end{array} & & \begin{array}{ c c }
    \text{b)} & \lim\limits _{n\rightarrow \infty }\left(\left(\frac{7+3n}{3n}\right)^{-n}\right)
  \end{array}
\end{align*}

\subsection*{LÃ¶sung 5}
Es gilt:

\begin{gather*}
  \lim _{n\rightarrow \infty }\left( 1+\frac{1}{n}\right)^{n} =e\\
  \lim _{n\rightarrow \infty }\left( 1-\frac{1}{n}\right)^{n} =e^{-1}
\end{gather*}

\subsubsection*{5a)}

\begin{equation*}
  \lim\limits _{n\rightarrow \infty }\left(\left( 1-\frac{2}{n}\right)^{3n}\right) =\lim\limits _{n\rightarrow \infty }\left(\left( 1-\frac{2}{n}\right)^{n}\right)^{3} =\left(\frac{1}{e^{2}}\right)^{3} =\frac{1}{e^{6}}
\end{equation*}

\subsubsection*{5b)}

\begin{equation*}
  \lim\limits _{n\rightarrow \infty }\left(\left(\frac{7+3n}{3n}\right)^{-n}\right) =\lim\limits _{n\rightarrow \infty }\left(\left(\frac{7+3n}{3n}\right)^{-n}\right) =\frac{1}{e^{\frac{7}{3}}}
\end{equation*}